\begin{flalign}
&\left| \overrightarrow {P}\right| =\sigma_{p} \left[ C/m^2\right]
\end{flalign}

\begin{flalign}
&E_{v}=\dfrac {\sigma _{t}}{\varepsilon _{0}}\left[ v/m\right]
\end{flalign}

\begin{flalign}
&E_{d}=\dfrac {\sigma _{t}-\sigma _{p}}{\varepsilon _{0}}\left[ V/m\right]
\end{flalign}

\begin{eqnarray}
\varepsilon _{0}&=&\dfrac {E_{v}}{\sigma _{t}}\left( \sigma _{t}-\sigma _{p}\right)\\
&=&\left( 1-\dfrac {\sigma _{p}}{\sigma _{t}}\right) E_{v}
\end{eqnarray}

\begin{eqnarray}
E_{d}&=&\dfrac {\sigma _{t}}{\varepsilon _{0}}-\dfrac {\sigma _{p}}{\varepsilon _{0}}\\
&=&E_{v}-\dfrac {1}{\varepsilon _{0}}P\\
&=&E^{\rightarrow _{v}}-\dfrac {1}{\varepsilon _{0}}\overrightarrow {P}\
\end{eqnarray}


\begin{flalign}
&C_{u}=\dfrac {\varepsilon _{0}S}{l}\left[ F\right]
\end{flalign}

\begin{eqnarray}
C_{d}&=&\dfrac {\varepsilon S}{l}\\
&=&\dfrac {\varepsilon _{s}\varepsilon _{0}S}{l}\left[ F\right]
\end{eqnarray}

\begin{flalign}
&C_{d}=\varepsilon _{s}C_{v}
\end{flalign}

\begin{eqnarray}
\dfrac {E_{d}}{E_{v}}&=&\dfrac {V_{d}/l}{V_{v}/l}=\dfrac {V_{d}}{V_{v}}\\
&=&\dfrac {Q/Cd}{Q/C_{v}}=\dfrac {C_{v}}{C_{d}}
\end{eqnarray}

\begin{flalign}
&\dfrac {E_{d}}{E_{v}}=\dfrac {C_{v}}{\varepsilon _{s}C_{v}}\\
&E_{d}=\dfrac {1}{\varepsilon _{s}}\cdot E_{v}
\end{flalign}

\begin{flalign}
&D_{v}=\varepsilon _{0}E_{v}
\end{flalign}

\begin{flalign}
&D_{d}=\varepsilon E_{d}
\end{flalign}

\begin{flalign}
&E_{d}=\dfrac {1}{\varepsilon _{s}}E_{v}\\
&\varepsilon _{s}E_{d}=E_{v}\\
&\varepsilon _{s}\varepsilon _{0}E_{d}=\varepsilon _{0}E_{v}\\
&D_{d}=D_{v}\left[ C/m^{2}\right]
\end{flalign}

\begin{flalign}
&E_{v}=\dfrac {\sigma _{t}}{\varepsilon _{0}}\\
&\varepsilon _{0}E_{v}=\sigma _{t}\\
&Dv=\sigma _{t}\left[ C/m^{2}\right]\\
&D_{d}=\sigma _{t}\left[ C/m^{2}\right]
\end{flalign}

\begin{flalign}
&F=\dfrac {Q_{1}Q_{2}}{4\pi \varepsilon r^{2}}\left[ N\right]
\end{flalign}

\begin{eqnarray}
W&=&\dfrac {1}{2}\varepsilon E^{2}\\
&=&\dfrac {1}{2}ED\left[ J/m^{3}\right]
\end{eqnarray}

\begin{eqnarray}
f&=&\dfrac {1}{2}\varepsilon E^{2}\\
&=&\dfrac {1}{2}ED\left[ N/m^{2}\right]
\end{eqnarray}

\begin{flalign}
&\theta _{1}\neq \theta _{2}
\end{flalign}

\begin{flalign}
&\oint Edl=0\\
&E_{it}\Delta l-E_{2t}\Delta l=0\\
&E_{1t}=E_{2t}
\end{flalign}
