\begin{flalign}
&\Delta H\propto I\\
&\Delta H\propto \Delta l\\
&\Delta H\propto \dfrac {1}{r^{2}}\\
&\Delta H\propto \dfrac {I\cdot \Delta l}{r^{2}}
\end{flalign}

\begin{flalign}
&\Delta H=\dfrac {1}{4\pi }\cdot \dfrac {I\cdot \Delta l}{r^{2}}
\end{flalign}

\begin{flalign}
&\Delta H=\dfrac {1}{4\pi }\dfrac {I\cdot \Delta l}{r^{2}}\sin \theta \left[ A/m\right]
\end{flalign}

\begin{flalign}
&\overrightarrow {a}\times \overrightarrow {b}
\end{flalign}

\begin{flalign}
&\left| \overrightarrow {a}\times \overrightarrow {b}\right| =\left| \overrightarrow {a}\right| \cdot \left| \overrightarrow {b}\right| \sin \theta
\end{flalign}

\begin{flalign}
&\left| \Delta \overrightarrow {l}\times \overrightarrow {r}\right| =\Delta l\cdot r\cdot \sin \theta
\end{flalign}

\begin{eqnarray}
\Delta H&=&\dfrac {1}{4\pi }\dfrac {I\cdot \Delta l}{r^{2}}\sin \theta \\
&=&\dfrac {I}{4\pi }\cdot \dfrac {\Delta lr\sin \theta }{r^{3}}\\
&=&\dfrac {I}{4\pi }\cdot \dfrac {\left| \Delta \overrightarrow {l}\times \overrightarrow {r}\right| }{r^{3}}
\end{eqnarray}

\begin{flalign}
&\Delta \overrightarrow {H}=\dfrac {I}{4\pi }\cdot \dfrac {\Delta \overrightarrow {l}\times \overrightarrow {r}}{r^{3}}\left[ A/m\right]
\end{flalign}

\begin{flalign}
&\overrightarrow {B}=\mu _{0}\overrightarrow {H}\left[ T\right] \\
&\mu _{0}=4\pi \times 10^{-7}\left[ H/m\right]
\end{flalign}

\begin{flalign}
&\Delta H=\dfrac {I\Delta x\sin \theta }{4\pi r^{2}}
\end{flalign}

\begin{flalign}
&\sin \theta =\dfrac {a}{r}\rightarrow r=\dfrac {a}{\sin \theta }\\
&\tan \theta =\dfrac {a}{x}\rightarrow x=\dfrac {a}{\tan \theta }
\end{flalign}

\begin{flalign}
&x=\dfrac {\cos \theta }{\sin \theta }a
\end{flalign}

\begin{eqnarray}
\dfrac {dx}{d\theta }&=&\dfrac {-\sin ^{2}\theta -\cos ^{2}\theta }{\sin ^{2}\theta }a\\
&=&-\dfrac {a}{\sin ^{2}\theta }
\end{eqnarray}

\begin{eqnarray}
H&=&\sum \Delta H\\
&=&\sum \dfrac {I\Delta x\sin \theta }{4\pi r^{2}}=\sum \dfrac {I \sin \theta}{4\pi r^{2}}\Delta x\\
&=&\int ^{\infty }_{-\infty}\dfrac {I\sin \theta }{4\pi r^{2}}dx\\
&=& \int ^{0}_{\pi }\dfrac { I \sin \theta }{4\pi \dfrac {a^{2}}{\sin ^{2}\theta }}\left( -\dfrac {a}{\sin ^{2}\theta }\right) d\theta\\
&=&\int ^{0}_{\pi }\dfrac {-I\sin \theta }{4\pi a}d\theta \\
&=&\dfrac {1}{4\pi a}\int ^{0}_{\pi }\left( -\sin \theta \right) d\theta \\
&=&\dfrac {1}{4\pi a}\left[ \cos \theta \right] ^{0}_{\pi }\\
&=&\dfrac {1}{4\pi a}\left( 1-\left( -1\right) \right) \\
&=&\dfrac {I}{2\pi a}\left[ A/m\right]
\end{eqnarray}

\begin{eqnarray}
H&=&\int ^{x_{2}}_{x_{1}}\dfrac {I\sin \theta }{4\pi r^{2}}dx\\
&=&\int ^{\alpha _{1}}_{\pi -\alpha _{2}}\dfrac {-I\sin \theta }{4\pi a}d\theta \\
&=&\dfrac {I}{4\pi a}\left[ \cos \theta \right] ^{\alpha _{1}}_{\pi -\alpha _{2}}\\
&=&\dfrac {I}{4\pi a}\left( \cos \alpha _{1}-\cos \left( \pi -\alpha _{2}\right) \right) \\
&=&\dfrac {I}{4\pi a}\left( \cos \alpha _{1}+\cos \alpha _{2}\right)\left[ A/m\right]
\end{eqnarray}

\begin{eqnarray}
H&=&4\times \dfrac {I}{4\pi \times \dfrac {l}{2}}\left( \cos \dfrac {\pi }{4}\times 2\right)\\
&=&2\dfrac {I}{\pi l}\left( \dfrac {2}{\sqrt {2}}\right) \\
&=&\dfrac {2\sqrt {2}I}{\pi l}\left[ A/m\right]
\end{eqnarray}

\begin{flalign}
&\sum ^{n}_{i=1}H_{i}\Delta l_{i}=H\cdot 2\pi a
\end{flalign}

\begin{flalign}
&H=\dfrac {I}{2\pi a}\left[ A/m\right] \\
&H\cdot 2\pi a=I\\
&\therefore \sum ^{n}_{i=1}H_{i}\cdot \Delta l_{i}=I
\end{flalign}

\begin{flalign}
&\oint _{C_{0}}Hdl=I
\end{flalign}

\begin{flalign}
&\oint _{C_{0}}\overrightarrow {H}\cdot \overrightarrow {t}dl=I\\
&\oint _{C_{0}}H\cos \theta dl=I
\end{flalign}

\begin{flalign}
&\oint _{C_{0}}Hdl=I\\
&H\cdot 2\pi r=I\\
&H=\dfrac {I}{2\pi r}\left[ A/m\right]
\end{flalign}

\begin{flalign}
&\oint _{C_{0}}Hdl=I\\
&H\cdot 2\pi r=I\\
&H=\dfrac {I}{2\pi r}\left[ A/m\right]
\end{flalign}

\begin{flalign}
&\dfrac {I}{\pi a^{2}}\times \pi r^{2}=I\dfrac {r^{2}}{a^{2}}\left[ A\right] \\
&\oint _{C_{0}}Hdl=I\dfrac {r^{2}}{a^{2}}\\
&H=\dfrac {Ir^{2}}{2\pi ra^{2}}\\
&H=\dfrac {Ir}{2\pi a^{2}}\left[ A/m\right]
\end{flalign}

\begin{flalign}
&\oint _{C_{0}}Hdl=NI\\
&H\times 2\pi a=NI\\
&H=\dfrac {NI}{2\pi a}\left[ A/m\right]
\end{flalign}

\begin{flalign}
&B=\mu _{0}H=\dfrac {\mu _{0}NI}{2\pi a}\left[ T\right] \left[ Wb/m^2\right]
\end{flalign}

\begin{flalign}
&\phi =BS=\dfrac {\mu _{0}NIS}{2\pi a}\left[ Wb\right]
\end{flalign}

\begin{flalign}
&\oint _{C_{1}}Hdl=0\\
&-H_{1}\times a+H_{2}\times a=0\\
&H_{1}=H_{2}
\end{flalign}

\begin{flalign}
&\oint _{C_{3}}Hdl=0\\
&H_{3}=H_{4}\\
&H_{3}=H_{4}=0\left[ A/m\right]
\end{flalign}

\begin{flalign}
&\oint _{C_{2}}Hdl=\left( na\right) I\\
&-H_{5}\times a+H_{6}\times a=naI\\
&0\times a+H_{6}\times a=naI\\
&H_{6}=nI\left[ A/m\right]
\end{flalign}

\begin{flalign}
&H=n\cdot I\left[ A/m\right]
\end{flalign}

\begin{eqnarray}
\Delta \phi &=& B \times c \Delta x\\
&=& \mu _{0}\dfrac {I}{2\pi x}c\Delta x
\end{eqnarray}

\begin{eqnarray}
\phi &=&\sum \Delta \phi \\
&=&\sum \dfrac {\mu _{0}Ic}{2\pi x}\Delta x\\
&=&\int ^{b}_{a}\dfrac {\mu _{0}Ic}{2\pi x}dx\\
&=&\dfrac {\mu _{0}Ic}{2\pi }\left[ \log \left| x\right| \right] ^{b}_{a}\\
&=&\dfrac {\mu _{0}Ic}{2\pi }\log \dfrac {b}{a}\left[ Wb\right]
\end{eqnarray}

\begin{flalign}
&F\propto I\\
&F\propto l\\
&F\propto B\\
&F\propto IBl
\end{flalign}

\begin{flalign}
&F=IlB\left[ N\right]
\end{flalign}

\begin{flalign}
&&F=Il(B \cdot \sin \theta)\left[ N\right]
\end{flalign}

\begin{flalign}
&Il = qv
\end{flalign}

\begin{flalign}
&F=IlB
&F=qvB
\end{flalign}

\begin{flalign}
&\overrightarrow {F}=\left( \overrightarrow {I}\times \overrightarrow {B}\right) l\\
&\overrightarrow {F}=\left( \overrightarrow {v}\times \overrightarrow {B}\right) q
\end{flalign}

\begin{flalign}
&T=rF
\end{flalign}

\begin{eqnarray}
T&=&\dfrac {a}{2}\times F\sin \theta \times 2\\
&=&aF\sin \theta \\
&=&abIB\sin \theta \left[ Nm\right]
\end{eqnarray}

\begin{flalign}
&T=SIB\sin \theta \left[ Nm\right]
\end{flalign}

\begin{flalign}
&T=SIB\sin \theta \left[ Nm\right]
\end{flalign}

\begin{flalign}
&m\alpha =F\\
m\dfrac {v^{2}}{r}=lVB\\
m\dfrac {v}{r}=eB\\
r=\dfrac {mv}{eB}\left[ m\right]
\end{flalign}

\begin{flalign}
&\omega =\dfrac {V}{r}=\dfrac {eB}{m}\left[ \mathrm{rad}/s\right]
\end{flalign}

\begin{flalign}
&n=\dfrac {\omega }{2\pi }=\dfrac {eB}{2\pi m}\left[ s^{-1}\right]
\end{flalign}

\begin{flalign}
&F_{2}=I_{2}lB,\\
&B_{1}=\mu _{0}H_{1}=\mu _{0}\dfrac {I_{1}}{2\pi a}\\
&F_{1}=\dfrac {\mu _{0}I_{1}I_{2}l}{2\pi a}\left[ N\right] \\
&F_{1}=F_{2}
\end{flalign}

\begin{flalign}
&E=vB\\
&J=qnv\left[ A/m^{2}\right] \\
&v=\dfrac {J}{qn}\left[ m/s\right] \\
&\therefore \cdot E=\dfrac {J}{qn}B\left[ V/m\right]
\end{flalign}

\begin{flalign}
&\dfrac {E}{J}=\dfrac {1}{qn}B\\
\end{flalign}

$\dfrac {1}{qn}$をホール定数といい，$R_H$とおく．

\begin{flalign}
&\dfrac {E}{J}=R_{H}\times B\\
&\therefore B=\dfrac {1}{R_{H}}\cdot \dfrac {V_{H}/d}{I/dl}\left[ T\right]
\end{flalign}

\begin{flalign}
&F=IlB\left[ N\right]
\end{flalign}

\begin{flalign}
&W=-F_x=-IlBx\left[ J\right]
\end{flalign}

\begin{flalign}
&\phi = BS = B\left( xl \right)
\end{flalign}

\begin{flalign}
&W=-I\phi \left[ J\right]
\end{flalign}
