\begin{flalign}
&e\propto \dfrac {\Delta \phi }{\Delta t}
\end{flalign}

\begin{flalign}
&e=-\dfrac {d\phi }{dt}\left[ N\right]
\end{flalign}

\begin{flalign}
&e=-n\dfrac {d\phi }{dt}\left[ N\right]
\end{flalign}

\begin{flalign}
&e=-\dfrac {d\psi }{dt}\left[ V\right]
\end{flalign}

\begin{flalign}
&\psi =n\phi \left[ Wb\right]
\end{flalign}

\begin{eqnarray}
e&=&-n\dfrac {d\phi }{dt}\\
&=&-n\dfrac {d}{dt}BS\\
&=&-n\dfrac {d}{dt}\left( B\left( y\cdot x\cdot \cos \theta \right) \right)
\end{eqnarray}

\begin{eqnarray}
e&=&-n\dfrac {d}{dt}\left( Byx\cos \omega t\right) \\
&=&-nBxy\left( -\sin \omega t\right) \cdot \omega \\
&=&n\omega xyB\sin \omega t \left[ V\right]
\end{eqnarray}

\begin{flalign}
&qE=\varepsilon vB\\
&E=v_{B}\left[ V/m\right]
\end{flalign}

\begin{flalign}
&e=vBl\left[ V\right]
\end{flalign}

\begin{flalign}
&\overrightarrow {e}=\left( \overrightarrow {v}\times \overrightarrow {B}\right) l\left[ V\right]
\end{flalign}

\begin{eqnarray}
W_{m}&=&F\times \left( v\times \Delta t\right) \\
&=&IlB\times v\times \Delta t\left[ J\right]
\end{eqnarray}

\begin{eqnarray}
W_{e}&=&e\times I\times \Delta t\\
&=&V\times B\times l\times I\times \Delta t\left[ J\right]
\end{eqnarray}

\begin{flalign}
&W_{m}=W_{e}
\end{flalign}
